Write a first version of xlet

lean/Cfml.lean
@@ -1,5 +1,231 @@
 import Lean
+import Cfml.Init
 
 namespace Cfml
+
+inductive Result (α : Type u) where
+  | ok (v: α): Result α
+  | fail : Result α
+deriving Repr, BEq
+
+open Result
+
+instance Result_Inhabited (α : Type u) : Inhabited (Result α) :=
+  Inhabited.mk fail
+
+instance Result_Nonempty (α : Type u) : Nonempty (Result α) :=
+  Nonempty.intro fail
+
+/- HELPERS -/
+
+def ok? {α: Type u} (r: Result α): Bool :=
+  match r with
+  | ok _ => true
+  | fail => false
+
+/- DO-DSL SUPPORT -/
+
+def bind {α : Type u} {β : Type v} (x: Result α) (f: α → Result β) : Result β :=
+  match x with
+  | ok v  => f v
+  | fail => fail
+
+-- Allows using Result in do-blocks
+instance : Bind Result where
+  bind := bind
+
+-- Allows using pure x in do-blocks
+instance : Pure Result where
+  pure := fun x => ok x
+
+@[simp] theorem bind_ok (x : α) (f : α → Result β) : bind (.ok x) f = f x := by simp [bind]
+@[simp] theorem bind_fail (f : α → Result β) : bind .fail f = .fail := by simp [bind]
+
+/- CUSTOM-DSL SUPPORT -/
+
+-- Let-binding the Result of a monadic operation is oftentimes not sufficient,
+-- because we may need a hypothesis for equational reasoning in the scope. We
+-- rely on subtype, and a custom let-binding operator, in effect recreating our
+-- own variant of the do-dsl
+
+def Result.attach {α: Type} (o : Result α): Result { x : α // o = ok x } :=
+  match o with
+  | ok x => ok ⟨x, rfl⟩
+  | fail => fail
+
+@[simp] theorem bind_tc_ok (x : α) (f : α → Result β) :
+  (do let y ← .ok x; f y) = f x := by simp [Bind.bind, bind]
+
+@[simp] theorem bind_tc_fail (x : Error) (f : α → Result β) :
+  (do let y ← fail; f y) = fail := by simp [Bind.bind, bind]
+
+@[simp] theorem bind_assoc_eq {a b c : Type u}
+  (e : Result a) (g :  a → Result b) (h : b → Result c) :
+  (Bind.bind (Bind.bind e g) h) =
+  (Bind.bind e (λ x => Bind.bind (g x) h)) := by
+  simp [Bind.bind]
+  cases e <;> simp
+
+def f (x : α) : Result α := do
+  let x ← ok x
+  ok x
+
+def double (x : Int) : Result Int := do
+  ok (x + x)
+
+def quadruple (x : Int) : Result Int := do
+  let y ← double x
+  double y
+
+def spec (r : Result α) (Q : α → Prop) : Prop :=
+  match r with
+  | ok v => Q v
+  | fail => false
+
+theorem spec_ok (v : α) (Q : α → Prop) (h : Q v) :
+  spec (ok v) Q := by
+  simp [spec, *]
+
+theorem spec_let e Q1 Q :
+  spec e Q1 →
+  (∀ x, Q1 x → spec (k x) Q) →
+  spec (bind e k) Q := by
+  simp [spec, bind, *]
+  cases e <;> simp
+  sorry
+
+-- TODO: ==>
+@[simp]
+def entails (Q1 Q2 : α → Prop) : Prop :=
+  ∀ x, Q1 x → Q2 x
+
+theorem refl_entails : entails Q Q := sorry
+
+theorem spec_weaken :
+  spec e Q1 →
+  entails Q1 Q2 →
+  spec e Q2 := by sorry
+
+-- TODO: notation =2*x
+theorem spec_double (x : Int) :
+  spec (double x) (λ y => y = 2 * x) :=
+  sorry
+
+theorem spec_quadruple (x : Int) :
+  spec (quadruple x) (λ y => y = 4 * x) := by
+  rw [quadruple]
+  apply spec_let
+  . apply spec_double
+  . intro y Hy
+    apply spec_weaken
+    apply spec_double; simp 
+    intro y Hy; simp_all
+    sorry
+  . apply spec_double
+  sorry
+
+theorem spec_quadruple1 (x : Int) :
+  spec (quadruple x) (λ y => y = 4 * x) := by
+  rw [quadruple]
+  apply spec_let
+  . apply spec_weaken
+    apply spec_double
+    apply refl_entails
+  . intro y Hy
+    apply spec_weaken
+    apply spec_double; simp 
+    intro y Hy; simp_all
+    sorry
+  . 
+    apply spec_double
+  sorry
+
+-- xlet
+-- xlet P
+-- xlet_val
+--syntax xletTac := ("as" " ⟨ " (ident <|> "_"),* " .."? " ⟩")?
+
+--def evalProgress (args : TSyntax `Progress.progressArgs) : TacticM Unit := do
+--  let args := args.raw
+
+set_option trace.Xlet true
+open Lean Elab Term Meta Tactic
+
+#check Expr
+
+#check LocalContext
+#check ConstantInfo
+#check Expr.const
+
+-- xlet
+-- xlet P
+-- xlet
+syntax xletArgs := (ident)?
+elab "xlet" args:xletArgs : tactic => do
+  -- Focus on the current goal
+  Tactic.focus do
+  withMainContext do
+  -- Retrieve the goal
+  let mgoal ← Tactic.getMainGoal
+  let goalTy ← mgoal.getType
+  trace[Xlet] "goal: {goalTy}"
+  -- Expected goal: spec (let x ← _; k) Q
+  -- Retrieve: (let x ← _; k)
+  goalTy.consumeMData.withApp fun _ args => do
+  let e := args.get! 1 -- bind _ (fun x => k x)
+  trace[Xlet] "e: {e}"
+  e.consumeMData.withApp fun _bind bindArgs => do
+  trace[Xlet] "bindArgs: {bindArgs}"
+  let k := bindArgs.get! 5
+  trace[Xlet] "k: {k}"
+  -- Dive into the lambda
+  lambdaTelescope k fun kArgs kBody => do
+  trace[Xlet] "k: {kArgs}"
+  -- Retrieve the first binder
+  let x := kArgs.get! 0
+  trace[Xlet] "x: {x}"
+  let xId := x.fvarId!
+  -- Lookup the name of the variable
+  let ctx ← Lean.MonadLCtx.getLCtx
+  let decl := ctx.get! xId
+  let yName :=
+    match decl with
+    | .cdecl _index _ userName _ _ _ => userName
+    | .ldecl _index _ userName _ _ _ _ => userName
+  trace[Xlet] "yName: {yName}"
+  -- Apply the theorem
+  let env ← getEnv
+  let thDecl := env.constants.find! ``spec_let
+  -- We have to introduce fresh meta-variables for the universes already
+  let ul : List Level ←
+    thDecl.levelParams.mapM (λ _ => do pure (← mkFreshLevelMVar))
+  let th := Expr.const ``spec_let ul
+  trace[Xlet] "th: {th}"
+  let ngoals ← mgoal.apply th
+  setGoals ngoals
+  -- intro y in the second goal
+  match ngoals with
+  | goal1 :: goal2 :: goals =>
+    let (_, ngoal2) ← goal2.intro yName
+    setGoals (goal1 :: ngoal2 :: goals)
+    pure ()
+  | _ =>
+    -- Error
+    panic "There should be at least 2 goals"
+
+/-
+-- TODO: use name given by lambda
+syntax "xlet" : tactic
+macro_rules
+  | `(tactic| xlet) =>
+    `(tactic|
+      apply spec_let; [|intro])
+-/
+
+theorem spec_quadruple2 (x : Int) :
+  spec (quadruple x) (λ y => y = 4 * x) := by
+  rw [quadruple]
+  xlet
+
 
 end Cfml
